rvcore: Update to match interface

examples/dynamic_isolation/RVCore.v
@@ -388,6 +388,8 @@ Module RV32Core (RVP: RVParams) (Multiplier: MultiplierInterface)
   Import ListNotations.
   Import RVP.
   Import Common.
+  Import Core_Common.
+
 
   Definition fetch_bookkeeping :=
     {| struct_name := "fetch_bookkeeping";
@@ -436,7 +438,7 @@ Module RV32Core (RVP: RVParams) (Multiplier: MultiplierInterface)
   End ScoreboardParams.
   Module Scoreboard := Scoreboard ScoreboardParams.
 
-  Inductive internal_reg_t' : Type :=
+  Inductive internal_reg_t :=
   | f2d (state: fromFetch.reg_t)
   | f2dprim (state: waitFromFetch.reg_t)
   | d2e (state: fromDecode.reg_t)
@@ -448,8 +450,6 @@ Module RV32Core (RVP: RVParams) (Multiplier: MultiplierInterface)
   | epoch
   | freeze_fetch
   .
-
-  Definition internal_reg_t := internal_reg_t'.
 
   Definition R_internal (idx: internal_reg_t) : type :=
     match idx with
@@ -479,66 +479,40 @@ Module RV32Core (RVP: RVParams) (Multiplier: MultiplierInterface)
     | freeze_fetch => Bits.zero
     end.
 
-  Inductive external_reg_t :=
-  | core_id
-  | toIMem (state: MemReq.reg_t)
-  | toDMem (state: MemReq.reg_t)
-  | fromIMem (state: MemResp.reg_t)
-  | fromDMem (state: MemResp.reg_t)
-  | toSMEnc (state: EnclaveReq.reg_t)
-  | rf (state: Rf.reg_t) 
-  | pc
-  | purge
-  .
+  Instance FiniteType_toIMem : FiniteType MemReq.reg_t := _.
+  Instance FiniteType_fromIMem : FiniteType MemResp.reg_t := _.
+  Instance FiniteType_toDMem : FiniteType MemReq.reg_t := _.
+  Instance FiniteType_fromDMem : FiniteType MemResp.reg_t := _.
+  Instance FiniteType_f2d : FiniteType fromFetch.reg_t := _.
+  Instance FiniteType_f2dprim : FiniteType waitFromFetch.reg_t := _.
+  Instance FiniteType_d2e : FiniteType fromDecode.reg_t := _.
+  Instance FiniteType_e2w : FiniteType fromExecute.reg_t := _.
+  Instance FiniteType_mulState : FiniteType Multiplier.reg_t := Multiplier.FiniteType_reg_t.
+  Instance FiniteType_rf : FiniteType Rf.reg_t := _.
+  Declare Instance FiniteType_scoreboard_rf : FiniteType Scoreboard.Rf.reg_t.
+  Instance FiniteType_scoreboard : FiniteType Scoreboard.reg_t := _.
+  Declare Instance FiniteType_internal_reg_t : FiniteType internal_reg_t. (* TODO *)
 
-  Definition R_external (idx: external_reg_t) : type :=
-    match idx with
-    | core_id => core_id_t
-    | toIMem r => MemReq.R r
-    | toDMem r => MemReq.R r
-    | fromIMem  r => MemResp.R r
-    | fromDMem  r => MemResp.R r
-    | toSMEnc r => EnclaveReq.R r
-    | rf r => Rf.R r  
-    | pc => bits_t 32
-    | purge => enum_t purge_state
-    end.  
+  Definition internal_params : internal_module_sig :=
+    {| _internal_reg_t := internal_reg_t;
+       _r_internal := r_internal;
+       _R_internal := R_internal;
+       _FiniteType_internal_reg_t := FiniteType_internal_reg_t
+    |}.
 
-  Definition r_external (idx: external_reg_t) : R_external idx :=
-    match idx with
-    | core_id => CoreParams.core_id
-    | toIMem s => MemReq.r s
-    | fromIMem s => MemResp.r s
-    | toDMem s => MemReq.r s
-    | fromDMem s => MemResp.r s
-    | toSMEnc s => EnclaveReq.r s
-    | rf r => Rf.r r  
-    | pc => CoreParams.initial_pc
-    | purge => value_of_bits (Bits.zero)
-    end.
+  Definition reg_t := @Core_Common.reg_t internal_params.
+  Definition r := @Core_Common.r CoreParams.core_id CoreParams.initial_pc internal_params.
+  Definition R := @Core_Common.R internal_params.
 
-  Inductive reg_t :=
-  | external (r: external_reg_t)
-  | internal (r: internal_reg_t)
-  .
+  Instance FiniteType_reg_t : FiniteType reg_t := @Core_Common.FiniteType_reg_t internal_params.
 
-  Definition R (idx: reg_t) : type :=
-    match idx with
-    | external r => R_external r
-    | internal r => R_internal r
-    end.
+  Definition ext_fn_t := @Core_Common.ext_fn_t External.ext.
+  Definition rule := @Core_Common.rule internal_params External.ext.
+  Definition sigma := @Core_Common.sigma External.ext.
+  Definition Sigma := @Core_Common.Sigma External.ext.
 
-  Definition r idx : R idx :=
-    match idx with
-    | external s => r_external s
-    | internal s => r_internal s
-    end.                              
-
-  Definition ext_fn_t := External.ext_fn_t.
-  Definition Sigma := External.Sigma.
-  Definition rule := rule R Sigma.
-  Definition sigma := External.sigma. 
-
+  Notation internal := (@internal internal_params).
+  Notation external := (@external internal_params).
   (* TODO *)
   Notation "'__external__' instance " :=
     (fun reg => external ((instance) reg)) (in custom koika at level 1, instance constr at level 99).
@@ -547,6 +521,7 @@ Module RV32Core (RVP: RVParams) (Multiplier: MultiplierInterface)
   Notation "'(' instance ').(' method ')' args" :=
     (USugar (UCallModule instance _ method args))
       (in custom koika at level 1, method constr, args custom koika_args at level 99).
+
 
   Definition fetch : uaction reg_t ext_fn_t :=
     {{
@@ -818,16 +793,6 @@ Module RV32Core (RVP: RVParams) (Multiplier: MultiplierInterface)
   | Purge.
 
   Definition rule_name_t := rule_name_t'.
-
-  Instance FiniteType_toIMem : FiniteType MemReq.reg_t := _.
-  Instance FiniteType_fromIMem : FiniteType MemResp.reg_t := _.
-  Instance FiniteType_toDMem : FiniteType MemReq.reg_t := _.
-  Instance FiniteType_fromDMem : FiniteType MemResp.reg_t := _.
-  Instance FiniteType_f2d : FiniteType fromFetch.reg_t := _.
-  Instance FiniteType_d2e : FiniteType fromDecode.reg_t := _.
-  Instance FiniteType_e2w : FiniteType fromExecute.reg_t := _.
-
-
   Instance Show_rf : Show (Rf.reg_t) :=
     { show '(Rf.rData v) := rv_register_name v }.
 
@@ -835,8 +800,10 @@ Module RV32Core (RVP: RVParams) (Multiplier: MultiplierInterface)
     { show '(Scoreboard.Scores (Scoreboard.Rf.rData v)) := rv_register_name v }.
 
   Existing Instance Multiplier.Show_reg_t.
-  Instance Show_reg_t : Show reg_t := _.
-  Instance Show_ext_fn_t : Show ext_fn_t := _.
+
+  (* TODO *)
+  (* Instance Show_reg_t : Show reg_t := _. *)
+  (* Instance Show_ext_fn_t : Show ext_fn_t := _. *)
 End RV32Core.
 
 (* Definition rv_external (rl: rv_rules_t) := false. *)
@@ -869,11 +836,14 @@ End Mul32Params.
 Module RV32I (EnclaveParams: EnclaveParameters) (CoreParams: CoreParameters)
              <: Core_sig External EnclaveParams CoreParams.
   Module Multiplier := ShiftAddMultiplier Mul32Params.
-  Include (RV32Core RV32IParams Multiplier EnclaveParams CoreParams).
-
-  (* TODO: needed for type checking *)
   Import External.
   Import Common.
+  Import Core_Common.
+
+  Include (RV32Core RV32IParams Multiplier EnclaveParams CoreParams).
+
+
+  (* TODO: needed for type checking *)
 
   Definition reset_scoreboard : UInternalFunction reg_t empty_ext_fn_t :=
     {{ fun reset_scoreboard () : bits_t 0 =>
@@ -949,7 +919,7 @@ Module RV32I (EnclaveParams: EnclaveParameters) (CoreParams: CoreParameters)
   Definition tc_writeback := tc_rule R Sigma writeback.
   Definition tc_step_multiplier := tc_rule R Sigma step_multiplier.
   Definition tc_tick := tc_rule R Sigma tick.
-  Definition tc_purge := tc_rule R Sigma do_internal_purge <: rule.
+  Definition tc_purge := tc_rule R Sigma do_internal_purge.
 
   Definition rules (rl: rule_name_t) : rule :=
     match rl with
@@ -966,240 +936,23 @@ Module RV32I (EnclaveParams: EnclaveParameters) (CoreParams: CoreParameters)
   Definition schedule : scheduler :=
     Writeback |> Execute |> StepMultiplier |> Decode |> WaitImem |> Fetch |> Tick |> Purge |> done.
 
-  Instance FiniteType_rf : FiniteType Rf.reg_t := _.
-  Instance FiniteType_scoreboard_rf : FiniteType Scoreboard.Rf.reg_t := _.
-  Instance FiniteType_scoreboard : FiniteType Scoreboard.reg_t := _.
-  Instance FiniteType_internal_reg_t : FiniteType internal_reg_t := _.
-  Instance FiniteType_ext_reg_t : FiniteType external_reg_t := _.
-  Instance FiniteType_reg_t : FiniteType reg_t := _.
+  (* Instance FiniteType_rf : FiniteType Rf.reg_t := _. *)
+  (* Instance FiniteType_scoreboard_rf : FiniteType Scoreboard.Rf.reg_t := _. *)
+  (* Instance FiniteType_scoreboard : FiniteType Scoreboard.reg_t := _. *)
+  (* Instance FiniteType_internal_reg_t : FiniteType internal_reg_t := _. *)
+  (* Instance FiniteType_ext_reg_t : FiniteType external_reg_t := _. *)
+  (* Instance FiniteType_reg_t : FiniteType reg_t := _. *)
 
-  Section CycleSemantics.
-    Definition state := env_t ContextEnv (fun idx : reg_t => R idx).
-    Definition empty_log : Log R ContextEnv := log_empty.
+  Parameter output_correctness : @P_output_correctness CoreParams.core_id CoreParams.initial_pc
+                                                        internal_params External.ext
+                                                        rule_name_t rules schedule.
 
-    Definition initial_state := ContextEnv.(create) r.
-
-    Parameter update_function : state -> Log R ContextEnv -> Log R ContextEnv.
-      (* interp_scheduler' st ? rules log scheduler. *)
-
-    Record step_io :=
-      { step_input : Log R_external ContextEnv;
-        step_feedback: Log R_external ContextEnv
-      }.
-
-    Definition lift_ext_log (log: Log R_external ContextEnv) : Log R ContextEnv :=
-      ContextEnv.(create) (fun reg => match reg return (RLog (R reg)) with
-                                   | external s => ContextEnv.(getenv) log s
-                                   | _ => []
-                                   end).
-
-    Definition do_step__koika (st: state) (step: step_io)
-                            : state * Log R ContextEnv :=
-      let input := lift_ext_log step.(step_input) in
-      let output := update_function st input in
-      let final := log_app (lift_ext_log step.(step_feedback)) (log_app output input) in
-      (commit_update st final, output).
-
-    Definition do_steps__koika (steps: list step_io) 
-                             : state * list (Log R ContextEnv) :=
-      fold_left (fun '(st, evs) step =>
-                   let '(st', ev) := do_step__koika st step in
-                   (st', evs ++ [ev]))
-                steps (initial_state, []).
-
-  End CycleSemantics.
-
-  Section Interface.
-    Definition proj_log__ext (log: Log R ContextEnv) : Log R_external ContextEnv :=
-      ContextEnv.(create) (fun reg => ContextEnv.(getenv) log (external reg)).
-
-      Definition tau := Log R_external ContextEnv.
-      Definition trace := list tau.
-  End Interface.
-
-  Section Spec.
-
-    Definition is_external_log (log: Log R ContextEnv) : Prop :=
-      forall reg, match reg with
-             | external r => True
-             | internal r => ContextEnv.(getenv) log reg = []
-             end.
-
-    (* TODO: to simplify for now, we say that the Core executes first *)
-    Definition valid_input_log__common (input_log: Log R_external ContextEnv) : Prop :=
-      input_log = log_empty.
-
-    Definition valid_output_log__common (output_log: Log R_external ContextEnv) : Prop :=
-      True.
-    
-    Definition valid_feedback_log__common (log: Log R_external ContextEnv) : Prop :=
-      (* Writeback to external registers only *)
-      latest_write log core_id = None /\
-      (* TODO: Register file is really internal... we just wanted to be able to talk about it *)
-      (forall s, latest_write log (rf s) = None).
-    (*
-      (latest_write log (external (toIMem MemReq.valid0)) = None \/
-      latest_write log (external (toIMem MemReq.valid0)) = Some Ob~0).
-      *)
-    
-    (* - While running, SM only gets to write purging (which doesn't change anything)
-     * - Only Core writes purged, transitioning from running -> waiting
-     * - Here, Core promises to not change external state
-     * - Supposing that SM writes restart only when external state is cleared (apart from certain regs),
-     * - Then simulation of resetting holds.
-     *)
-    Inductive phase_state :=
-    | SpecSt_Running
-    | SpecSt_Waiting (rf: env_t ContextEnv Rf.R)
-    .
-
-    Definition spec_state_t : Type := state * phase_state.
-
-    Definition initial_spec_state : spec_state_t := (initial_state, SpecSt_Running).
-
-    Definition only_write_ext_purge (log: Log R_external ContextEnv) (v: bits_t 2) : Prop :=
-      latest_write log purge = Some v \/ latest_write log purge = None.
-
-    Definition only_write_purge (log: Log R ContextEnv) (v: bits_t 2) : Prop :=
-      latest_write log (external purge) = Some v \/ latest_write log (external purge) = None.
-
-    Definition extract_rf (st: state) : env_t ContextEnv Rf.R :=
-      ContextEnv.(create) (fun reg => ContextEnv.(getenv) st (external (rf reg))).
-    
-    Definition initialise_with_rf (initial_rf: env_t ContextEnv Rf.R) (initial_pc: bits_t 32) : state :=
-      ContextEnv.(create) (fun reg => match reg return R reg with
-                                   | external (rf s) => ContextEnv.(getenv) initial_rf s
-                                   | external pc => initial_pc
-                                   | s => r s
-                                   end).
-    
-    (* TODO: should really be inductive probably or option type? But too much effort to specify everything. *)
-    Definition do_step_trans__spec (spec_st: spec_state_t) (step: step_io)
-                                 : spec_state_t * Log R_external ContextEnv :=
-      let '(st, phase) := spec_st in
-      let '(st', output) := do_step__koika st step in
-      let ext_output := proj_log__ext output in 
-      match phase with
-      | SpecSt_Running =>
-          let continue := ((st', SpecSt_Running), ext_output) in
-          match latest_write output (external purge) with
-          | Some v => if bits_eqb v ENUM_purge_purged 
-                     then ((st', SpecSt_Waiting (extract_rf st')), ext_output)
-                     else continue
-          | None => continue
-          end
-      | SpecSt_Waiting _rf => 
-         let continue := ((st', SpecSt_Waiting _rf), ext_output) in
-         match latest_write step.(step_feedback) purge,
-               latest_write step.(step_feedback) pc with
-         | Some v, Some _pc => 
-             if bits_eqb v ENUM_purge_restart then
-               (((initialise_with_rf _rf _pc), SpecSt_Running), ext_output)
-             else (* don't care *) continue
-         | _, _ => continue
-         end
-      end.
-
-    (* Behaves nicely with enq/deqs *)
-    Definition valid_interface_log (st: state) (init_log: Log R_external ContextEnv) 
-                                   (log: Log R_external ContextEnv) : Prop. Admitted.
-
-    Definition no_writes (log: Log R_external ContextEnv) : Prop :=
-      forall r, latest_write log r = None.
-
-    Definition valid_step_output__spec (spec_st: spec_state_t) (step: step_io) : Prop :=
-      let '(st, phase) := spec_st in
-      let '(st', log) := do_step_trans__spec spec_st step in
-      valid_output_log__common log /\
-      valid_interface_log st log_empty log  /\
-        (match phase with
-        | SpecSt_Running => True
-        | SpecSt_Waiting _ =>
-            no_writes log
-        end).
-
-    Definition reset_external_state (st: state) : Prop :=
-      forall reg, match reg with
-             | rf _ => True
-             | pc => True
-             | purge => True
-             | s => ContextEnv.(getenv) st (external s) = r_external s
-             end.
-
-    Definition valid_step_feedback__spec (spec_st: spec_state_t) (step: step_io) : Prop :=
-      let '(st, phase) := spec_st in
-      let '(st', output) := do_step_trans__spec spec_st step in
-      let feedback := step.(step_feedback) in
-
-      valid_feedback_log__common step.(step_feedback) /\
-      valid_interface_log st (log_app output step.(step_input)) feedback /\
-      match phase with
-      | SpecSt_Running =>
-          only_write_ext_purge feedback ENUM_purge_purging
-      | SpecSt_Waiting _  =>
-          only_write_ext_purge feedback ENUM_purge_restart /\
-          (latest_write feedback purge = Some ENUM_purge_restart ->
-           latest_write feedback pc <> None /\
-           reset_external_state (fst st') (* TODO: whose responsibility to clear FIFOs? *)
-          )
-      end.
-
-    Definition do_step__spec (spec_st: spec_state_t) (step: step_io)
-                           : spec_state_t * Log R_external ContextEnv * props_t :=
-      let '(st', log) := do_step_trans__spec spec_st step in
-      let props' := {| P_input := valid_input_log__common step.(step_input);
-                       P_output := valid_step_output__spec spec_st step;
-                       P_feedback := valid_step_feedback__spec spec_st step
-                    |} in
-      (st', log, props').
-
-    Definition do_steps__spec (steps: list step_io) 
-                            : spec_state_t * list (Log R_external ContextEnv) * list props_t :=
-      fold_left (fun '(st, evs, props) step => 
-                   let '(st', ev, prop) := do_step__spec st step in
-                   (st', evs ++ [ev], props ++ [prop]))
-                steps (initial_spec_state, [], []).
-     
-  End Spec.
-
-  Section Correctness.
-
-    (* TODO: clean *)
-    Definition log_equivalent (koika_log: Log R ContextEnv) (spec_log: Log R_external ContextEnv) : Prop :=
-      forall (reg: external_reg_t), 
-        latest_write koika_log (external reg) = latest_write spec_log reg /\
-        (forall port, may_read koika_log port (external reg) = may_read spec_log port reg) /\
-        (forall port, may_write koika_log log_empty port (external reg) =
-                 may_write spec_log log_empty port reg).
-
-    Definition trace_equivalent (koika_tr: list (Log R ContextEnv)) 
-                                (spec_tr: list (Log R_external ContextEnv)) : Prop :=
-      Forall2 log_equivalent koika_tr spec_tr.
-
-    Axiom correctness :
-      forall (steps: list step_io) 
-        (spec_st: spec_state_t) (spec_tr: list (Log R_external ContextEnv)) (props: list props_t)
-        (koika_st: state) (koika_tr: list (Log R ContextEnv)),
-      valid_inputs props ->
-      valid_feedback props ->
-      do_steps__spec steps = (spec_st, spec_tr, props) ->
-      do_steps__koika steps = (koika_st, koika_tr) ->
-      trace_equivalent koika_tr spec_tr.
-
-  End Correctness.
-
-  Section Compliance.
-    Axiom compliance:
-      forall (steps: list step_io) 
-        (spec_st: spec_state_t) (spec_tr: list (Log R_external ContextEnv)) (props: list props_t)
-        (koika_st: state) (koika_tr: list (Log R ContextEnv)),
-      valid_inputs props ->
-      valid_feedback props ->
-      do_steps__spec steps = (spec_st, spec_tr, props) ->
-      do_steps__koika steps = (koika_st, koika_tr) ->
-      valid_output props.
-
-  End Compliance.
+  Parameter correctness : @P_correctness CoreParams.core_id CoreParams.initial_pc
+                                         internal_params External.ext
+                                         rule_name_t rules schedule.
+  Parameter compliance : @P_compliance CoreParams.core_id CoreParams.initial_pc
+                                       internal_params External.ext
+                                       rule_name_t rules schedule.
 
 End RV32I.
 
